Initial QED for Impl.Blake2.Incremental

code/blake2b/experimental/Hacl.Impl.Blake2b.Incremental.fst
@@ -178,7 +178,7 @@ let blake2b_incremental_update_first block pl ll input =
  (* /\ i * Spec.size_block Spec.Blake2B <= Seq.length input /\ init + (i * Spec.size_block Spec.Blake2B) <= Spec.max_limb Spec.Blake2B}) *)
 noextract
 let spec_incremental_update_loop_step
-  (init:size_nat)
+  (state:SpecI.state_r Spec.Blake2B)
   (ni:size_nat)
   (ll:size_nat)
   (input:LBS.lbytes ll{ni * Spec.size_block Spec.Blake2B <= Seq.length input})
@@ -188,7 +188,7 @@ let spec_incremental_update_loop_step
   let block: Spec.block_s Spec.Blake2B =
     Seq.sub #uint8 #(Seq.length input) input (i * (Spec.size_block Spec.Blake2B)) (Spec.size_block Spec.Blake2B)
   in
-  Spec.blake2_update_block Spec.Blake2B (init + (i * Spec.size_block Spec.Blake2B)) block hash
+  Spec.blake2_update_block Spec.Blake2B ((state.SpecI.n * Spec.size_block Spec.Blake2B) + (i * Spec.size_block Spec.Blake2B)) block hash
 
 
 inline_for_extraction noextract
@@ -208,7 +208,7 @@ val blake2b_incremental_update_loop_step:
   (ensures  fun h0 _ h1 ->
     modifies1 state.hash h0 h1 /\
     state_inv h1 state /\
-    h1.[|state.hash|] == spec_incremental_update_loop_step (v (gstate_get_n h0 state) * Spec.size_block Spec.Blake2B) (v ni) (v ni * Spec.size_block Spec.Blake2B) h0.[|blocks|] (v i) h0.[|state.hash|])
+    h1.[|state.hash|] == spec_incremental_update_loop_step (spec_of h0 state) (v ni) (v ni * Spec.size_block Spec.Blake2B) h0.[|blocks|] (v i) h0.[|state.hash|])
 
 inline_for_extraction noextract
 let blake2b_incremental_update_loop_step state ni i blocks =
@@ -224,17 +224,17 @@ let blake2b_incremental_update_loop_step state ni i blocks =
 
 noextract
 val spec_blake2_incremental_update_loop:
-  init:size_nat
-  -> blocks:LBS.bytes{Seq.length blocks <= max_size_t /\ Seq.length blocks % (Spec.size_block Spec.Blake2B) = 0 /\ (init + (Seq.length blocks / (Spec.size_block Spec.Blake2B))) * (Spec.size_block Spec.Blake2B) < pow2 128}
+  (state:SpecI.state_r Spec.Blake2B)
+  -> blocks:LBS.bytes{Seq.length blocks <= max_size_t /\ Seq.length blocks % (Spec.size_block Spec.Blake2B) = 0 /\ ((state.SpecI.n * Spec.size_block Spec.Blake2B) + (Seq.length blocks / (Spec.size_block Spec.Blake2B))) * (Spec.size_block Spec.Blake2B) < pow2 128}
   -> hash:Spec.hash_ws Spec.Blake2B ->
   Tot (Spec.hash_ws Spec.Blake2B)
 
 noextract
-let spec_blake2_incremental_update_loop init blocks hash =
-  let n = Seq.length blocks / Spec.size_block Spec.Blake2B in
-  repeati n (fun i hash ->
-    spec_incremental_update_loop_step init n (n * Spec.size_block Spec.Blake2B) blocks i hash
-  ) hash
+let spec_blake2_incremental_update_loop state blocks hash =
+  let ni = Seq.length blocks / Spec.size_block Spec.Blake2B in
+  [@inline_let]
+  let spec = spec_incremental_update_loop_step state ni (ni * Spec.size_block Spec.Blake2B) blocks in
+  repeati ni spec hash
 
 
 inline_for_extraction noextract
@@ -254,18 +254,18 @@ val blake2b_incremental_update_loop:
   (ensures  fun h0 _ h1 ->
     modifies1 state.hash h0 h1 /\
     state_inv h1 state /\
-    h1.[|state.hash|] == spec_blake2_incremental_update_loop (v ni) h0.[|blocks|] h0.[|state.hash|])
+    h1.[|state.hash|] == spec_blake2_incremental_update_loop (spec_of h0 state) h0.[|blocks|] h0.[|state.hash|])
 
 inline_for_extraction noextract
 let blake2b_incremental_update_loop state ni blocks =
   let h0 = ST.get () in
   [@inline_let]
-  let spec h = spec_incremental_update_loop_step (v (gstate_get_n h0 state) * Spec.size_block Spec.Blake2B) (v ni) (v ni * Spec.size_block Spec.Blake2B) h.[|blocks|] in
+  let spec h = spec_incremental_update_loop_step (spec_of h0 state) (v ni) (v ni * Spec.size_block Spec.Blake2B) h.[|blocks|] in
   loop1 h0 ni state.hash spec
   (fun i ->
     Loops.unfold_repeati (v ni) (spec h0) h0.[|state.hash|] (v i);
-    blake2b_incremental_update_loop_step state ni i blocks);
-  admit()
+    blake2b_incremental_update_loop_step state ni i blocks
+  )
 
 
 noextract
@@ -279,7 +279,6 @@ val spec_blake2_incremental_update_end:
 
 noextract
 let spec_blake2_incremental_update_end block ll ll0 ll2 input =
-  (* let ll2 = (ll - ll0) % (Spec.size_block Spec.Blake2B) in *)
   let input2 = Seq.sub #uint8 #ll input (ll - ll2) ll2 in
   Seq.update_sub block 0 ll2 input2
 
@@ -394,7 +393,7 @@ let spec_blake2b_incremental_update_inner_longer2 ll input state rb ll0 =
   let open Spec.Blake2.Incremental in
   let n1 = (ll - ll0) / Spec.size_block Spec.Blake2B in
   let input1 = Seq.sub #uint8 #ll input ll0 (n1 * Spec.size_block Spec.Blake2B) in
-  let hash = spec_blake2_incremental_update_loop state.n input1 state.hash in
+  let hash = spec_blake2_incremental_update_loop state input1 state.hash in
   let state = {state with hash = hash; n = state.SpecI.n + n1;} in
   state
 
@@ -413,6 +412,7 @@ val blake2b_incremental_update_inner_longer2:
     disjoint state.hash input /\ disjoint state.block input /\
     disjoint state.n input /\ disjoint state.pl input /\
     v (gstate_get_n h state) + (v ll - v ll0) / v size_block <= max_size_t /\
+    v (gstate_get_n h state) * v size_block <= max_size_t /\
     v (gstate_get_n h state) * (v size_block) + v ll < pow2 128)
   (ensures  fun h0 _ h1 ->
     modifies3 state.hash state.block state.n h0 h1 /\
@@ -510,7 +510,7 @@ let spec_blake2b_incremental_update_inner_longer ll input state rb ll0 =
   (* Handle all full blocks available *)
   let n1 = (ll - ll0) / Spec.size_block Spec.Blake2B in
   let input1 = Seq.sub #uint8 #ll input ll0 (n1 * Spec.size_block Spec.Blake2B) in
-  let hash = spec_blake2_incremental_update_loop state.n input1 state.hash in
+  let hash = spec_blake2_incremental_update_loop state input1 state.hash in
   let state = {state with hash = hash; n = state.SpecI.n + n1;} in
   (* Store the remainder *)
   let ll2 = (ll - ll0) % Spec.size_block Spec.Blake2B in
@@ -546,6 +546,7 @@ val blake2b_incremental_update_inner_longer:
     disjoint state.n input /\ disjoint state.pl input /\
     state_inv h state /\
     v (gstate_get_n h state) + 1 + (v ll / v size_block) <= max_size_t /\
+    (v (gstate_get_n h state) + 1) * v size_block <= max_size_t /\
     v (gstate_get_n h state) * (v size_block) + v ll < pow2 128)
   (ensures  fun h0 _ h1 ->
     modifies4 state.hash state.block state.n state.pl h0 h1 /\
@@ -593,6 +594,7 @@ val blake2b_incremental_update_inner:
     v (gstate_get_pl h state) + v ll0 <= v size_block /\
     v rb = v size_block - v (gstate_get_pl h state) /\ v rb <= v size_block /\
     v (gstate_get_n h state) + 1 + v ll / v size_block <= max_size_t /\
+    (v (gstate_get_n h state) + 1) * v size_block <= max_size_t /\
     v (gstate_get_n h state) * (v size_block) + v ll < pow2 128)
   (ensures  fun h0 _ h1 ->
     modifies4 state.hash state.block state.n state.pl h0 h1 /\
@@ -678,6 +680,7 @@ val blake2b_incremental_update:
     disjoint state.n input /\ disjoint state.pl input /\
     state_inv h state /\
     v (gstate_get_n h state) + 2 + v ll / v size_block <= max_size_t /\
+    (v (gstate_get_n h state) + 1) * v size_block <= max_size_t /\
     v (gstate_get_n h state) * (v size_block) + v ll < pow2 128)
   (ensures  fun h0 b h1 ->
     state_inv h1 state /\
